Define reorderability (stronger)

State.v
@@ -90,6 +90,10 @@ End Stack.
 
 Module Config.
 
+Section CONFIG.
+
+Variable md:Ir.IRModule.t.
+
 (* Definition of a program state. *)
 Structure t := mk
   {
@@ -97,7 +101,6 @@ Structure t := mk
     s:Stack.t; (* a call stack *)
     cid_to_f:list (Ir.callid * nat); (*callid -> function id*)
     cid_fresh: Ir.callid; (* Fresh, unused call id. *)
-    md:Ir.IRModule.t (* IR module *)
   }.
 
 (* Wellformedness of a program state. *)
@@ -113,13 +116,13 @@ Structure wf (c:t) := mk_wf
     (* wf_cid_to_f2: All function ids in cid_to_f are valid, i.e.,
        has corresponding function definition. *)
     wf_cid_to_f2: forall cf (HIN:List.In cf c.(cid_to_f)),
-        exists f, Ir.IRModule.getf cf.(snd) c.(md) = Some f;
+        exists f, Ir.IRModule.getf cf.(snd) md = Some f;
     (* wf_stack: all PCs stored in the call stack (which is c.(s))
        are valid, respective to corresponding functions. *)
     wf_stack: forall curcid curpc funid f curregfile
                      (HIN:List.In (curcid, (curpc, curregfile)) c.(s))
                      (HIN2:List.In (curcid, funid) c.(cid_to_f))
-                     (HF:Some f = Ir.IRModule.getf funid c.(md)),
+                     (HF:Some f = Ir.IRModule.getf funid md),
         Ir.IRFunction.valid_pc curpc f = true
     (* WIP - more properties will be added later. *)
   }.
@@ -149,12 +152,12 @@ Definition update_rval (c:t) (regid:nat) (v:Ir.val): t :=
   match c.(s) with
   | nil => c
   | (cid, (pc0, r))::s' =>
-    mk c.(m) ((cid, (pc0, Regfile.update r regid v))::s') c.(cid_to_f) c.(cid_fresh) c.(md)
+    mk c.(m) ((cid, (pc0, Regfile.update r regid v))::s') c.(cid_to_f) c.(cid_fresh)
   end.
 
 (* Update memory. *)
 Definition update_m (c:t) (m:Ir.Memory.t): t :=
-  mk m c.(s) c.(cid_to_f) c.(cid_fresh) c.(md).
+  mk m c.(s) c.(cid_to_f) c.(cid_fresh).
 
 (* Get function id (= function name) of cid. *)
 Definition get_funid (c:t) (cid:Ir.callid): option nat :=
@@ -166,17 +169,17 @@ Definition get_funid (c:t) (cid:Ir.callid): option nat :=
 (* Update PC into next_pc. *)
 Definition update_pc (c:t) (next_pc:Ir.IRFunction.pc): t :=
   match c.(s) with
-  | (cid, (pc0, r))::t => mk c.(m) ((cid,(next_pc, r))::t) c.(cid_to_f) c.(cid_fresh) c.(md)
+  | (cid, (pc0, r))::t => mk c.(m) ((cid,(next_pc, r))::t) c.(cid_to_f) c.(cid_fresh)
   | _ => c
   end.
 
 (* Get (definition of the running function, PC inside the function). *)
 Definition cur_fdef_pc (c:t): option (Ir.IRFunction.t * Ir.IRFunction.pc) :=
-  match (Ir.Config.s c) with
+  match (s c) with
   | (cid, (pc0, _))::t =>
-    match Ir.Config.get_funid c cid with
+    match get_funid c cid with
     | Some funid =>
-      match Ir.IRModule.getf funid c.(md) with
+      match Ir.IRModule.getf funid md with
       | Some fdef => Some (fdef, pc0)
       | None => None
       end
@@ -194,18 +197,15 @@ Definition cur_inst (c:t): option (Ir.Inst.t) :=
 
 (* Returns true if the call stack has more than one entry, false otherwise. *)
 Definition has_nestedcall (c:t): bool :=
-  Nat.ltb 1 (List.length (Ir.Config.s c)).
+  Nat.ltb 1 (List.length (s c)).
 
 
 (* Definition of equality. *)
-(*     m:Ir.Memory.t; (* a memory *)
-    s:Stack.t; (* a call stack *)
-    cid_to_f:list (Ir.callid * nat); (*callid -> function id*)
-    cid_fresh: Ir.callid; (* Fresh, unused call id. *)
-    md:Ir.IRModule.t (* IR module *)*)
 Definition eq (c1 c2:t): Prop :=
   c1.(m) = c2.(m) /\ Stack.eq c1.(s) c2.(s) /\ c1.(cid_to_f) = c2.(cid_to_f) /\
-  c1.(cid_fresh) = c2.(cid_fresh) /\ c1.(md) = c2.(md).
+  c1.(cid_fresh) = c2.(cid_fresh).
+
+End CONFIG.
 
 End Config.
 
